\chapter{Equivalence of Indexing Specifications}\label{chapter:indexing}

\equivalencetheorem*

\begin{proof}~
{\scriptsize
\begin{itemize}
\item[$\Rightarrow$]
By simultaneous induction:
\begin{enumerate}
\item
Assume $\deduce{\Hoare{\Env = \Xi}{\IndexesKind{K}{\tilde K}}{\Env = \Xi'}}{\D}$.
\par
By structural induction on $\D$:
\begin{itemize}
\item
Case $\D = \infer{
	\Hoare{\Env = \Xi}{\IndexesKind{A \to K}{\tilde A \to \tilde K}}{\Env = \Unshift{\Psi}{\Xi'''}}
}{
	\deduce{\Hoare{\Env = \Xi}{\IndexesType{A}{\tilde A}}{\Env = \Xi''}}{\D_1}
	& \deduce{\Hoare{\Env = \Shift{\Psi}{\Xi''}}{\IndexesKind{K}{\tilde K}}{\Env = \Xi'''}}{\D_2}
}$.
\par
By the induction hypothesis on $\D_1$, we have $\deduce{\Xi \vdash \IndexesType{A}{\tilde A}}{\E_1}$ and $\Xi'' = \Xi$.
\par
By the induction hypothesis on $\D_2$, we have $\deduce{\Shift{\Psi}{\Xi''} \vdash \IndexesKind{K}{\tilde K}}{\E_2}$ and $\Xi''' = \Shift{\Psi}{\Xi''}$.
\par
Then, $\Xi' = \Unshift{\Psi}{\Xi'''} = \Unshift{\Psi}{\Shift{\Psi}{\Xi''}} = \Xi'' = \Xi$, and
\begin{equation*}
\infer{
	\Xi \vdash \IndexesKind{A \to K}{\tilde A \to \tilde K}
}{
	\deduce{\Xi \vdash \IndexesType{A}{\tilde A}}{\E_1}
	& \infer{\Xi, \_ : \LFTerm \vdash \IndexesKind{K}{\tilde K}}{\deduce{\Shift{\Psi}{\Xi} \vdash \IndexesKind{K}{\tilde K}}{\E_2}}
}.
\end{equation*}

\item
Case $\D = \infer{
	\Hoare{\Env = \Xi}{\IndexesKind{\Pi x{:}A. K}{\Pi_{\tilde A} \tilde K}}{\Env = \Pop{\Psi}{x}{\Xi'''}}
}{
	\deduce{\Hoare{\Env = \Xi}{\IndexesType{A}{\tilde A}}{\Env = \Xi''}}{\D_1}
	& \deduce{\Hoare{\Env = \Push{\Psi}{x : \LFTerm}{\Xi''}}{\IndexesKind{K}{\tilde K}}{\Env = \Xi'''}}{\D_2}
}$.
\par
By the induction hypothesis on $\D_1$, we have $\deduce{\Xi \vdash \IndexesType{A}{\tilde A}}{\E_1}$ and $\Xi'' = \Xi$.
\par
By the induction hypothesis on $\D_2$, we have $\deduce{\Push{\Psi}{x : \LFTerm}{\Xi''} \vdash \IndexesKind{K}{\tilde K}}{\E_2}$ and $\Xi''' = \Push{\Psi}{x : \LFTerm}{\Xi''}$.
\par
Then, $\Xi' = \Pop{\Psi}{x}{\Xi'''} = \Pop{\Psi}{x}{\Push{\Psi}{x : \LFTerm}{\Xi''}} = \Xi'' = \Xi$, and
\begin{equation*}
\infer{
	\Xi \vdash \IndexesKind{\Pi x{:}A. K}{\Pi_{\tilde A}\ \tilde K}
}{
	\deduce{\Xi \vdash \IndexesType{A}{\tilde A}}{\E_1}
	& \infer{\Xi, x : \LFTerm \vdash \IndexesKind{K}{\tilde K}}{\deduce{\Push{\Psi}{x : \LFTerm}{\Xi} \vdash \IndexesKind{K}{\tilde K}}{\E_2}}
}.
\end{equation*}

\item
Case $\D = \infer{
	\Hoare{\Env = \Xi}{\IndexesKind{\KWType}{\KWType}}{\Env = \Xi}
}{}$.
\par
$\Xi \vdash \IndexesKind{\KWType}{\KWType}$ holds trivially.
\end{itemize}
\item
Assume $\deduce{\Hoare{\Env = \Xi}{\IndexesType{A}{\tilde A}}{\Env = \Xi'}}{\D}$.
\par
By structural induction on $\D$:
\begin{itemize}
\item
Case $\D = \infer{
	\Hoare{\Env = \Xi}{\IndexesType{A \to B}{\tilde A \to \tilde B}}{\Env = \Unshift{\Psi}{\Xi'''}}
}{
	\deduce{\Hoare{\Env = \Xi}{\IndexesType{A}{\tilde A}}{\Env = \Xi''}}{\D_1}
	& \deduce{\Hoare{\Env = \Shift{\Psi}{\Xi''}}{\IndexesType{B}{\tilde B}}{\Env = \Xi'''}}{\D_2}
}$.
\par
By the induction hypothesis on $\D_1$, we have $\deduce{\Xi \vdash \IndexesType{A \to B}{\tilde A \to \tilde B}}{\E_1}$ and $\Xi'' = \Xi$.
\par
By the induction hypothesis on $\D_2$, we have $\deduce{\Shift{\Psi}{\Xi''} \vdash \IndexesType{B}{\tilde B}}{\E_2}$ and $\Xi''' = \Shift{\Psi}{\Xi''}$.
\par
Then, $\Xi' = \Unshift{\Psi}{\Xi'''} = \Unshift{\Psi}{\Shift{\Psi}{\Xi''}} = \Xi'' = \Xi$, and
\begin{equation*}
\infer{
	\Xi \vdash \IndexesType{A \to B}{\tilde A \to \tilde B}
}{
	\deduce{\Xi \vdash \IndexesType{A \to B}{\tilde A \to \tilde B}}{\E_1}
	& \infer{
		\Xi, \_ : \LFTerm \vdash \IndexesType{B}{\tilde B}
	}{
		\deduce{\Shift{\Psi}{\Xi} \vdash \IndexesType{B}{\tilde B}}{\E_2}
	}
}.
\end{equation*}

\item
Case $\D = \infer{
	\Hoare{\Env = \Xi}{\IndexesType{\Pi x{:}A. B}{\Pi_{\tilde A}\ \tilde B}}{\Env = \Pop{\Psi}{x}{\Xi'''}}
}{
	\deduce{\Hoare{\Env = \Xi}{\IndexesType{A}{\tilde A}}{\Env = \Xi''}}{\D_1}
	& \deduce{\Hoare{\Env = \Push{\Psi}{x : \LFTerm}{\Xi''}}{\IndexesType{B}{\tilde B}}{\Env = \Xi'''}}{\D_2}
}$.
\par
By the induction hypothesis on $\D_1$, we have $\deduce{\Xi \vdash \IndexesType{A}{\tilde A}}{\E_1}$ and $\Xi'' = \Xi$.
\par
By the induction hypothesis on $\D_2$, we have $\deduce{\Push{\Psi}{x : \LFTerm}{\Xi''} \vdash \IndexesType{B}{\tilde B}}{\E_2}$ and $\Xi''' = \Push{\Psi}{x : \LFTerm}{\Xi''}$.
\par
Then, $\Xi' = \Pop{\Psi}{x}{\Xi'''} = \Pop{\Psi}{x}{\Push{\Psi}{x : \LFTerm}{\Xi''}} = \Xi'' = \Xi$, and
\begin{equation*}
\infer{
	\Xi \vdash \IndexesType{\Pi x{:}A. B}{\Pi_{\tilde A}\ \tilde B}
}{
	\deduce{\Xi \vdash \IndexesType{A}{\tilde A}}{\E_1}
	& \infer{
		\Xi, x : \LFTerm \vdash \IndexesType{B}{\tilde B}
	}{
		\deduce{\Push{\Psi}{x : \LFTerm}{\Xi} \vdash \IndexesType{B}{\tilde B}}{\E_2}
	}
}.
\end{equation*}

\item
Case $\D = \infer{
	\Hoare{\Env = \Xi}{\IndexesType{a}{\tilde a}}{\Env = \Xi}
}{
	\deduce{\Lookup{a}{\Xi} = \tilde a : \LFTypeConst}{\D'}
}$.
\par
Then,
\begin{equation*}
\infer{
	\Xi \vdash \IndexesType{a}{\tilde a}
}{
	\deduce{\Lookup{a}{\Xi} = \tilde a : \LFTypeConst}{\D'}
}.
\end{equation*}

\item
Case $\D = \infer{
	\Hoare{\Env = \Xi}{\IndexesType{A\ M_1\ M_2 \dots M_n}{\tilde A\ \tilde M_1\ \tilde M_2 \dots \tilde M_n}}{\Env = \Xi_n}
}{
	\deduce{\Hoare{\Env = \Xi}{\IndexesType{A}{\tilde A}}{\Env = \Xi_0}}{\D_0}
	& \deduce{\left(\Hoare{\Env = \Xi_{k - 1}}{\IndexesTerm{M_k}{\tilde M_k}}{\Env = \Xi_k}\right)_{k \in \set{1, 2, \dots, n}}}{\D_2}
}$.
\par
By the induction hypothesis on $\D_0$, we have $\deduce{\Xi \vdash \IndexesType{A}{\tilde A}}{\E_0}$ and $\Xi_0 = \Xi$.
\par
For each $k \in \set{1, 2, \dots, n}$, by the induction hypothesis on $\D_k$, we have $\deduce{\Xi_{k - 1} \vdash \IndexesTerm{M_k}{\tilde M_k}}{\E_k}$ and $\Xi_{k - 1} = \Xi_k$.
\par
Then, inductively on $n$, we have $\Xi_n = \Xi_{n - 1} = \cdots = \Xi_0 = \Xi$, and
\begin{equation*}
\infer{
	\Xi \vdash \IndexesType{A\ M_1\ M_2 \dots M_n}{\tilde A\ \tilde M_1\ \tilde M_2 \dots \tilde M_n}
}{
	\deduce{\Xi \vdash \IndexesType{A}{\tilde A}}{\E_0}
	& \left(\deduce{\Xi \vdash \IndexesTerm{M_k}{\tilde M_k}}{\E_k}\right)_{k \in \set{1, 2, \dots, n}}
}.
\end{equation*}

\end{itemize}
\item
Assume $\deduce{\Hoare{\Env = \Xi}{\IndexesTerm{M}{\tilde M}}{\Env = \Xi'}}{\D}$.
\par
By structural induction on $\D$:
\begin{itemize}
\item
Case $\D = \infer{
	\Hoare{\Env = \Xi}{\IndexesTerm{x}{\iota}}{\Env = \Xi}
}{
	\deduce{\Lookup{x}{\Xi} = x : \LFTerm}{\D_1}
	& \deduce{\Index{\Psi}{x}{\Xi} = \iota}{\D_2}
}$.
\par
Then,
\begin{equation*}
\infer{
	\Xi \vdash \IndexesTerm{x}{\iota}
}{
	\deduce{\Lookup{x}{\Xi} = x : \LFTerm}{\D_1}
	& \deduce{\Index{\Psi}{x}{\Xi} = \iota}{\D_2}
}.
\end{equation*}

\item
Case $\D = \infer{
	\Hoare{\Env = \Xi}{\IndexesTerm{c}{\tilde c}}{\Env = \Xi}
}{
	\deduce{\Lookup{c}{\Xi} = \tilde c : \LFTermConst}{\D'}
}$.
\par
Then,
\begin{equation*}
\infer{
	\Xi \vdash \IndexesTerm{c}{\tilde c}
}{
	\deduce{\Lookup{c}{\Xi} = \tilde c : \LFTermConst}{\D'}
}.
\end{equation*}

\item
Case $\D = \infer{
	\Hoare{\Env = \Xi}{\IndexesTerm{\lambda x. M}{\lambda\ \tilde M}}{\Env = \Pop{\Psi}{x}{\Xi''}}
}{
	\deduce{\Hoare{\Env = \Push{\Psi}{x : \LFTerm}{\Xi}}{\IndexesTerm{M}{\tilde M}}{\Env = \Xi''}}{\D'}
}$.
\par
By the induction hypothesis on $\D'$, we have $\deduce{\Push{\Psi}{x : \LFTerm}{\Xi} \vdash \IndexesTerm{M}{\tilde M}}{\E'}$ and $\Xi'' = \Push{\Psi}{x : \LFTerm}{\Xi}$.
\par
Then, $\Xi' = \Pop{\Psi}{x}{\Xi''} = \Pop{\Psi}{x}{\Push{\Psi}{x : \LFTerm}{\Xi}} = \Xi$, and
\begin{equation*}
\infer{
	\Xi \vdash \IndexesTerm{\lambda x. M}{\lambda\ \tilde M}
}{
	\infer{
		\Xi, x : \LFTerm \vdash \IndexesTerm{M}{\tilde M}
	}{
		\deduce{\Push{\Psi}{x : \LFTerm}{\Xi} \vdash \IndexesTerm{M}{\tilde M}}{\E'}
	}
}.
\end{equation*}

\item
Case $\D = \infer{
	\Hoare{\Env = \Xi}{\IndexesTerm{M\ N_1\ N_2 \dots N_n}{\tilde M\ \tilde N_1\ \tilde N_2 \dots \tilde N_n}}{\Env = \Xi_n}
}{
	\deduce{\Hoare{\Env = \Xi}{\IndexesTerm{M}{\tilde M}}{\Env = \Xi_0}}{\D_0}
	& \left(\deduce{\Hoare{\Env = \Xi_{k - 1}}{\IndexesTerm{N_k}{\tilde N_k}}{\Env = \Xi_k}}{\D_k}\right)_{k \in \set{1, 2, \dots, n}}
}$.
\par
By the induction hypothesis on $\D_0$, we have $\deduce{\Xi \vdash \IndexesTerm{M}{\tilde M}}{\E_0}$ and $\Xi_0 = \Xi$.
\par
For each $k \in \set{1, 2, \dots, n}$, by the induction hypothesis on $\D_k$, we have $\deduce{\Xi_{k - 1} \vdash \IndexesTerm{N_k}{\tilde N_k}}{\E_k}$ and $\Xi_k = \Xi_{k - 1}$.
\par
Then, inductively on $n$, we have $\Xi_n = \Xi_{n - 1} = \cdots = \Xi_0 = \Xi$, and
\begin{equation*}
\infer{
	\Xi \vdash \IndexesType{M\ N_1\ N_2 \dots N_n}{\tilde M\ \tilde N_1\ \tilde N_2 \dots \tilde N_n}
}{
	\deduce{\Xi_{k - 1} \vdash \IndexesTerm{N_k}{\tilde N_k}}{\E_k}
	& \left(\deduce{\Xi \vdash \IndexesTerm{N_k}{\tilde N_k}}{\E_k}\right)_{k \in \set{1, 2, \dots, n}}
}.
\end{equation*}

\item
Case $\D = \infer{
	\Hoare{\Env = \Xi}{\IndexesTerm{M : A}{\tilde M : \tilde A}}{\Env = \Xi'}
}{
	\deduce{\Hoare{\Env = \Xi}{\IndexesTerm{M}{\tilde M}}{\Env = \Xi''}}{\D_1}
	& \deduce{\Hoare{\Env = \Xi''}{\IndexesType{A}{\tilde A}}{\Env = \Xi'}}{\D_2}
}$.
\par
By the induction hypothesis on $\D_1$, we have $\deduce{\Xi \vdash \IndexesTerm{M}{\tilde M}}{\E_1}$ and $\Xi'' = \Xi$.
\par
By the induction hypothesis on $\D_2$, we have $\deduce{\Xi'' \vdash \IndexesType{A}{\tilde A}}{\E_2}$ and $\Xi' = \Xi''$.
\par
Then, $\Xi' = \Xi'' = \Xi$, and
\begin{equation*}
\infer{
	\Xi \vdash \IndexesType{M : A}{\tilde M : \tilde A}
}{
	\deduce{\Xi \vdash \IndexesTerm{M}{\tilde M}}{\E_1}
	& \deduce{\Xi \vdash \IndexesType{A}{\tilde A}}{\E_2}
}.
\end{equation*}
\end{itemize}
\end{enumerate}
\item[$\Leftarrow$]
By simultaneous induction:
\begin{enumerate}
\item
Assume $\deduce{\Xi \vdash \IndexesKind{K}{\tilde K}}{\D}$.
\par
By structural induction on $\D$:
\begin{itemize}
\item
Case $\D = \infer{
	\Xi \vdash \IndexesKind{A \to K}{\tilde A \to \tilde K}
}{
	\deduce{\Xi \vdash \IndexesType{A}{\tilde A}}{\D_1}
	& \deduce{\Xi, \_ : \LFTerm \vdash \IndexesKind{K}{\tilde K}}{\D_2}
}$.
\par
By the induction hypothesis on $\D_1$, we have $\deduce{\Hoare{\Env = \Xi}{\IndexesType{A}{\tilde A}}{\Env = \Xi}}{\E_1}$.
\par
By the induction hypothesis on $\D_2$, we have $\deduce{\Hoare{\Env = \Xi, \_ : \LFTerm}{\IndexesKind{K}{\tilde K}}{\Env = \Xi, \_ : \LFTerm}}{\E_2}$.
\par
Then,
\begin{equation*}
\infer{
	\Hoare{\Env = \Xi}{\IndexesKind{A \to K}{\tilde A \to \tilde K}}{\Env = \Xi}
}{
	\infer{
		\Hoare{\Env = \Xi}{\IndexesKind{A \to K}{\tilde A \to \tilde K}}{\Env = \Unshift{\Psi}{\Shift{\Psi}{\Xi}}}
	}{
		\deduce{\Hoare{\Env = \Xi}{\IndexesType{A}{\tilde A}}{\Env = \Xi}}{\E_1}
		& \infer{\Hoare{\Env = \Shift{\Psi}{\Xi}}{\IndexesKind{K}{\tilde K}}{\Env = \Shift{\Psi}{\Xi}}}{\deduce{\Hoare{\Env = \Xi, \_ : \LFTerm}{\IndexesKind{K}{\tilde K}}{\Env = \Xi, \_ : \LFTerm}}{\E_2}}
	}
}.
\end{equation*}

\item
Case $\D = \infer{
	\Xi \vdash \IndexesKind{\Pi x{:}A. K}{\Pi_{\tilde A}\ \tilde K}
}{
	\deduce{\Xi \vdash \IndexesType{A}{\tilde A}}{\D_1}
	& \deduce{\Xi, x : \LFTerm \vdash \IndexesKind{K}{\tilde K}}{\D_2}
}$.
\par
By the induction hypothesis on $ \D_1 $, we have $ \deduce{\Hoare{\Env = \Xi}{\IndexesType{A}{\tilde A}}{\Env = \Xi}}{\E_1} $.
\par
By the induction hypothesis on $ \D_2 $, we have $ \deduce{\Hoare{\Env = \Xi, x : \LFTerm}{\IndexesKind{K}{\tilde K}}{\Env = \Xi, x : \LFTerm}}{\E_2} $.
\par
Then,
\begin{equation*}
\infer{
	\Hoare{\Env = \Xi}{\IndexesKind{\Pi x{:}A. K}{\Pi_{\tilde A} \tilde K}}{\Env = \Xi}
}{
\infer{
	\Hoare{\Env = \Xi}{\IndexesKind{\Pi x{:}A. K}{\Pi_{\tilde A} \tilde K}}{\Env = \Pop{\Psi}{x}{\Push{\Psi}{x : \LFTerm}{\Xi}}}
}{
	\deduce{\Hoare{\Env = \Xi}{\IndexesType{A}{\tilde A}}{\Env = \Xi}}{\E_1}
	& \infer{\Hoare{\Env = \Push{\Psi}{x : \LFTerm}{\Xi}}{\IndexesKind{K}{\tilde K}}{\Env = \Push{\Psi}{x : \LFTerm}{\Xi}}}{\deduce{\Hoare{\Env = \Xi, x : \LFTerm}{\IndexesKind{K}{\tilde K}}{\Env = \Xi, x : \LFTerm}}{\E_2}}
}
}.
\end{equation*}

\item
Case $\D = \infer{
	\Xi \vdash \IndexesKind{\KWType}{\KWType}
}{}$.
\par
$ \Hoare{\Env = \Xi}{\IndexesKind{\KWType}{\KWType}}{\Env = \Xi} $ holds trivially.
\end{itemize}
\item
Assume $\deduce{\Xi \vdash \IndexesType{A}{\tilde A}}{\D}$.
By structural induction on $\D$:
\begin{itemize}
\item
Case $\D = \infer{
	\Xi \vdash \IndexesType{A \to B}{\tilde A \to \tilde B}
}{
	\deduce{\Xi \vdash \IndexesType{A}{\tilde A}}{\D_1}
	& \deduce{\Xi, \_ : \LFTerm \vdash \IndexesType{B}{\tilde B}}{\D_2}
}$.
\par
By the induction hypothesis on $\D_1$, we have $\deduce{\Hoare{\Env = \Xi}{\IndexesType{A}{\tilde A}}{\Env = \Xi}}{\E_1}$.
\par
By the induction hypothesis on $\D_2$, we have $\deduce{\Hoare{\Env = \Xi, \_ : \LFTerm}{\IndexesType{B}{\tilde B}}{\Env = \Xi, \_ : \LFTerm}}{\E_2}$.
\par
Then,
\begin{equation*}
\infer{
	\Hoare{\Env = \Xi}{\IndexesType{A \to B}{\tilde A \to \tilde B}}{\Env = \Xi}
}{
	\infer{
		\Hoare{\Env = \Xi}{\IndexesType{A \to B}{\tilde A \to \tilde B}}{\Env = \Unshift{\Psi}{\Shift{\Psi}{\Xi}}}
	}{
		\deduce{\Hoare{\Env = \Xi}{\IndexesType{A}{\tilde A}}{\Env = \Xi}}{\E_1}
		& \infer{
			\Hoare{\Env = \Shift{\Psi}{\Xi}}{\IndexesType{B}{\tilde B}}{\Env = \Shift{\Psi}{\Xi}}
		}{
			\deduce{\Hoare{\Env = \Xi, \_ : \LFTerm}{\IndexesType{B}{\tilde B}}{\Env = \Xi, \_ : \LFTerm}}{\E_2}
		}
	}
}
.
\end{equation*}

\item
Case $\D = \infer{
	\Xi \vdash \IndexesType{\Pi x{:}A. B}{\Pi_{\tilde A}\ \tilde B}
}{
	\deduce{\Xi \vdash \IndexesType{A}{\tilde A}}{\D_1}
	& \deduce{\Xi, x : \LFTerm \vdash \IndexesType{B}{\tilde B}}{\D_2}
}$.
\par
By the induction hypothesis on $\D_1$, we have $\deduce{\Hoare{\Env = \Xi}{\IndexesType{A}{\tilde A}}{\Env = \Xi}}{\E_1}$.
\par
By the induction hypothesis on $\D_2$, we have $\deduce{\Hoare{\Env = \Xi, x : \LFTerm}{\IndexesType{B}{\tilde B}}{\Env = \Xi, x : \LFTerm}}{\E_2}$.
\par
Then,
\begin{equation*}
\infer{
	\Hoare{\Env = \Xi}{\IndexesType{\Pi x{:}A. B}{\Pi_{\tilde A}\ \tilde B}}{\Env = \Xi}
}{
	\infer{
		\Hoare{\Env = \Xi}{\IndexesType{\Pi x{:}A. B}{\Pi_{\tilde A}\ \tilde B}}{\Env = \Pop{\Psi}{x}{\Push{\Psi}{x : \LFTerm}{\Xi}}}
	}{
		\deduce{\Hoare{\Env = \Xi}{\IndexesType{A}{\tilde A}}{\Env = \Xi}}{\E_1}
		& \infer{
			\Hoare{\Env = \Push{\Psi}{x : \LFTerm}{\Xi}}{\IndexesType{B}{\tilde B}}{\Env = \Push{\Psi}{x : \LFTerm}{\Xi}}
		}{
			\deduce{\Hoare{\Env = \Xi, x : \LFTerm}{\IndexesType{B}{\tilde B}}{\Env = \Xi, x : \LFTerm}}{\E_2}
		}
	}
}.
\end{equation*}

\item
Case $\D = \infer{
	\Xi \vdash \IndexesType{a}{\tilde a}
}{
	\deduce{\Lookup{a}{\Xi} = \tilde a : \LFTypeConst}{\D'}
}$.
\par
Then,
\begin{equation*}
\infer{
	\Hoare{\Env = \Xi}{\IndexesType{a}{\tilde a}}{\Env = \Xi}
}{
	\deduce{\Lookup{a}{\Xi} = \tilde a : \LFTypeConst}{\D'}
}.
\end{equation*}

\item
Case $\D = \infer{
	\Xi \vdash \IndexesType{A\ M_1\ M_2 \dots M_n}{\tilde A\ \tilde M_1\ \tilde M_2 \dots \tilde M_n}
}{
	\deduce{\Xi \vdash \IndexesType{A}{\tilde A}}{\D_0}
	& \left(\deduce{\Xi \vdash \IndexesTerm{M_k}{\tilde M_k}}{\D_k}\right)_{k \in \set{1, 2, \dots, n}}
}$.
\par
By the induction hypothesis on $\D_0$, we have $\deduce{\Hoare{\Env = \Xi}{\IndexesType{A}{\tilde A}}{\Env = \Xi}}{\E_0}$.
\par
For each $k \in \set{1, 2, \dots, n}$, by the induction hypothesis on $\D_k$, we have $\deduce{\Hoare{\Env = \Xi}{\IndexesTerm{M_k}{\tilde M_k}}{\Env = \Xi}}{\E_k}$.
\par
Then,
\begin{equation*}
\infer{
	\Hoare{\Env = \Xi}{\IndexesType{A\ M_1\ M_2 \dots M_n}{\tilde A\ \tilde M_1\ \tilde M_2 \dots \tilde M_n}}{\Env = \Xi}
}{
	\deduce{\Hoare{\Env = \Xi}{\IndexesType{A}{\tilde A}}{\Env = \Xi}}{\E_0}
	& \left(\deduce{\Hoare{\Env = \Xi}{\IndexesTerm{M_k}{\tilde M_k}}{\Env = \Xi}}{\E_k}\right)_{k \in \set{1, 2, \dots, n}}
}.
\end{equation*}

\end{itemize}
\item
Assume $\deduce{\Xi \vdash \IndexesTerm{M}{\tilde M}}{\D}$.
\par
By structural induction on $\D$:
\begin{itemize}
\item
Case $\D = \infer{
	\Xi \vdash \IndexesTerm{x}{\iota}
}{
	\deduce{\Lookup{x}{\Xi} = x : \LFTerm}{\D_1}
	& \deduce{\Index{\Psi}{x}{\Xi} = \iota}{\D_2}
}$.
\par
Then,
\begin{equation*}
\infer{
	\Hoare{\Env = \Xi}{\IndexesTerm{x}{\iota}}{\Env = \Xi}
}{
	\deduce{\Lookup{x}{\Xi} = x : \LFTerm}{\D_1}
	& \deduce{\Index{\Psi}{x}{\Xi} = \iota}{\D_2}
}.
\end{equation*}

\item
Case $\D = \infer{
	\Xi \vdash \IndexesTerm{c}{\tilde c}
}{
	\deduce{\Lookup{c}{\Xi} = \tilde c : \LFTermConst}{\D'}
}$.
\par
Then,
\begin{equation*}
\infer{
	\Hoare{\Env = \Xi}{\IndexesTerm{c}{\tilde c}}{\Env = \Xi}
}{
	\deduce{\Lookup{c}{\Xi} = \tilde c : \LFTermConst}{\D'}
}.
\end{equation*}

\item
Case $\D = \infer{
	\Xi \vdash \IndexesTerm{\lambda x. M}{\lambda\ \tilde M}
}{
	\deduce{\Xi, x : \LFTerm \vdash \IndexesTerm{M}{\tilde M}}{\D'}
}$.
\par
By the induction hypothesis on $\D'$, we have $\deduce{\Hoare{\Env = \Xi, x : \LFTerm}{\IndexesTerm{M}{\tilde M}}{\Env = \Xi, x : \LFTerm}}{\E'}$.
\par
Then,
\begin{equation*}
\infer{
	\Hoare{\Env = \Xi}{\IndexesTerm{\lambda x. M}{\lambda\ \tilde M}}{\Env = \Xi}
}{
	\infer{
		\Hoare{\Env = \Xi}{\IndexesTerm{\lambda x. M}{\lambda\ \tilde M}}{\Env = \Pop{\Psi}{x}{\Push{\Psi}{x : \LFTerm}{\Xi}}}
	}{
		\infer{
		\Hoare{\Env = \Push{\Psi}{x : \LFTerm}{\Xi}}{\IndexesTerm{M}{\tilde M}}{\Env = \Push{\Psi}{x : \LFTerm}{\Xi}}
		}{
			\deduce{\Hoare{\Env = \Xi, x : \LFTerm}{\IndexesTerm{M}{\tilde M}}{\Env = \Xi, x : \LFTerm}}{\E'}
		}
	}
}.
\end{equation*}

\item
Case $\D = \infer{
	\Xi \vdash \IndexesType{M\ N_1\ N_2 \dots N_n}{\tilde M\ \tilde N_1\ \tilde N_2 \dots \tilde N_n}
}{
	\deduce{\Xi \vdash \IndexesTerm{M}{\tilde M}}{\D_0}
	& \left(\deduce{\Xi \vdash \IndexesTerm{N_k}{\tilde N_k}}{\D_k}\right)_{k \in \set{1, 2, \dots, n}}
}$.
\par
By the induction hypothesis on $\D_0$, we have $\deduce{\Hoare{\Env = \Xi}{\IndexesTerm{M}{\tilde M}}{\Env = \Xi}}{\E_0}$.
\par
For each $k \in \set{1, 2, \dots, n}$, by the induction hypothesis on $\D_k$, we have $\deduce{\Hoare{\Env = \Xi}{\IndexesTerm{N_k}{\tilde N_k}}{\Env = \Xi}}{\E_k}$.
\par
Then,
\begin{equation*}
\infer{
	\Hoare{\Env = \Xi}{\IndexesTerm{M\ N_1\ N_2 \dots N_n}{\tilde M\ \tilde N_1\ \tilde N_2 \dots \tilde N_n}}{\Env = \Xi}
}{
	\deduce{\Hoare{\Env = \Xi}{\IndexesTerm{M}{\tilde M}}{\Env = \Xi}}{\E_0}
	& \left(\deduce{\Hoare{\Env = \Xi}{\IndexesTerm{N_k}{\tilde N_k}}{\Env = \Xi}}{\E_k}\right)_{k \in \set{1, 2, \dots, n}}
}.
\end{equation*}

\item
Case $\D = \infer{
	\Xi \vdash \IndexesType{M : A}{\tilde M : \tilde A}
}{
	\deduce{\Xi \vdash \IndexesTerm{M}{\tilde M}}{\D_1}
	& \deduce{\Xi \vdash \IndexesType{A}{\tilde A}}{\D_2}
}$.
\par
By the induction hypothesis on $\D_1$, we have $\deduce{\Hoare{\Env = \Xi}{\IndexesTerm{M}{\tilde M}}{\Env = \Xi}}{\E_1}$.
\par
By the induction hypothesis on $\D_2$, we have $\deduce{\Hoare{\Env = \Xi}{\IndexesType{A}{\tilde A}}{\Env = \Xi}}{\E_2}$.
\par
Then,
\begin{equation*}
\infer{
	\Hoare{\Env = \Xi}{\IndexesTerm{M : A}{\tilde M : \tilde A}}{\Env = \Xi}
}{
	\deduce{\Hoare{\Env = \Xi}{\IndexesTerm{M}{\tilde M}}{\Env = \Xi}}{\E_1}
	& \deduce{\Hoare{\Env = \Xi}{\IndexesType{A}{\tilde A}}{\Env = \Xi}}{\E_2}
}.
\end{equation*}
\end{itemize}
\end{enumerate}
\end{itemize}
}
\end{proof}
