\noindent $ \boxed{\Xi \vdash \ucorner{M} \rightsquigarrow_M M' \dashv \Xi'} $ \quad The parser object $ \ucorner{M} $ is disambiguated to the \LF term $ M' $ under the disambiguation context $ \Xi $, which produces the output disambiguation state $ \Xi' $.

\begin{equation}
\infer{\Xi \vdash \ucorner{x} \rightsquigarrow_M x \dashv \Xi}{(x : \mathsf{LF}_{\mathsf{term}}) \in \Xi}
\end{equation}

\begin{equation}
\infer{\Xi \vdash \ucorner{c} \rightsquigarrow_M c \dashv \Xi}{(c : \mathsf{LF}_{\mathsf{term}}) \in \Xi}
\end{equation}

\begin{equation}
\infer{\Xi \vdash \ucorner{\lambda x {:} A. M} \rightsquigarrow_M \lambda x {:} A. M \dashv \Xi}{\Xi \vdash \ucorner{A }\rightsquigarrow_A A \dashv \Xi & \Xi, x : \mathsf{LF}_{\mathsf{term}} \vdash \ucorner{M} \rightsquigarrow M \dashv \Xi}
\end{equation}

\begin{equation}
\infer{\Xi \vdash \ucorner{M \; M_1 \; M_2 \; \dots \; M_n} \rightsquigarrow_M M \; M_1 \; M_2 \; \dots \; M_n \dashv \Xi}{\Xi \vdash \ucorner{M} \rightsquigarrow_M M \dashv \Xi & (\Xi \vdash \ucorner{M_i} \rightsquigarrow_M M_i \dashv \Xi)_{i \in \{1, 2, \dots, n\}}}
\end{equation}

\begin{equation}
\infer{\Xi \vdash \ucorner{M : A} \rightsquigarrow_M M : A \dashv \Xi}{\Xi \vdash \ucorner{M} \rightsquigarrow_M M \dashv \Xi & \Xi \vdash \ucorner{A} \rightsquigarrow_A A \dashv \Xi}
\end{equation}
